Added a new library from Mario Carneiro supporting "bit matches" of the kind often found in machine instruction decoding where words are decomposed into bitfields for casewise matching. This not only supports parsing and printing of such expressions with intuitive syntax
 `bitmatch w:int32 with
    [sf; op; S; 0b100010:6; sh; imm12:12; Rn:5; Rd:5] -> Rn
  | [sf; op; S; 0b01011000:8; Rm:5; 0:6; Rn:5; Rd:5] -> Rn`;;

but also provides efficient proof tools for manipulating such
expressions, e.g. bm_seq_numeral

 # bm_seq_numeral
   `bitmatch w:byte with
      [hi3:3; 0b00:2; lo3:3] -> foo hi3 lo3
    | [hi3:3; 0b1:1; lo4:4]  -> bar hi3 lo4
    | [0b1010101:7; b]       -> baz b`
    (Int 17);;

 val it : term * thm =
  (`word 17`,
   |- (bitmatch word 17 with
        [hi3:3; 0:2; lo3:3] -> foo hi3 lo3
      | [hi3:3; 1:1; lo4:4] -> bar hi3 lo4
      | [85:7; b] -> baz b) =
      bar (word 0) (word 1))

and BITMATCH_SEQ_CONV:

 # BITMATCH_SEQ_CONV
    `bitmatch (word 289406645 :int32) with
       [sf; op; S; 0b100010:6; sh; imm12:12; Rn:5; Rd:5] -> Rn
     | [sf; op; S; 0b01011000:8; Rm:5; 0:6; Rn:5; Rd:5] -> Rn`;;

  val it : thm =
  |- (bitmatch word 289406645 with
       [sf; op; S; 34:6; sh; imm12:12; Rn:5; Rd:5] -> Rn
     | [sf; op; S; 88:8; Rm:5; 0:6; Rn:5; Rd:5] -> Rn) =
     word 21

Also added some additional supporting lemmas to the core arithmetic
theories:

        BIT0_0
        BIT1_0
        EXP_2_NE_0
        MOD_DIV_EQ_0

and more word-related material: two new constants "numbit" (analogous
to "bit" but over :num not :N word) and "num_shift_add" (for
decomposing numerals along powers of 2):

        numbit
        num_shift_add

together with additional lemmas:

        num_shift_add_0
        num_shift_add_SUC
        num_shift_add_lt
        num_shift_add_mod

and supporting proof tools

        BIT_PRED
        NUMBIT_CONV
        NUM_SHIFT_ADD_CORE
        NUM_SHIFT_ADD_CONV

Library/words.ml
@@ -27,6 +27,9 @@
 (*  - WORD_RULE for simple algebraic properties                              *)
 (*  - WORD_BITWISE_RULE for bitwise-type properties of logical operations    *)
 (*  - WORD_ARITH for things involving numerical values                       *)
+(*                                                                           *)
+(*              (c) Copyright, John Harrison 2019-2020                       *)
+(*                (c) Copyright, Mario Carneiro 2020                         *)
 (* ========================================================================= *)
 
 let HAS_SIZE_8 = HAS_SIZE_DIMINDEX_RULE `:8`;;
@@ -921,6 +924,170 @@ let INT_REM_IVAL = prove
   POP_ASSUM MP_TAC THEN
   SIMP_TAC[LE_EXISTS; INT_POW_ADD; LEFT_IMP_EXISTS_THM] THEN
   REPEAT STRIP_TAC THEN CONV_TAC INTEGER_RULE);;
+
+(* ------------------------------------------------------------------------- *)
+(* Bit operations on `num`.                                                  *)
+(* ------------------------------------------------------------------------- *)
+
+let numbit = new_definition `numbit i n = ODD(n DIV (2 EXP i))`;;
+
+let NUMBIT_VAL = prove (`numbit i (val (e:N word)) = bit i e`,
+  REWRITE_TAC [numbit; BIT_VAL]);;
+
+(* * BIT_PRED `i` returns (None, `|- i = _0`) or (Some(`j`), `|- i = SUC j`)
+     if `i` is a raw numeral (a numeral without the initial `NUMERAL`).
+   * NUMBIT_CONV `numbit n i` proves `numbit n i = T` or `numbit n i = F` if
+     `n` and `i` are numerals or raw numerals. *)
+
+let BIT_PRED, NUMBIT_CONV =
+  let i,j,n,B0,B1 = `i:num`,`j:num`,`n:num`,`BIT0`,`BIT1` in
+  let B00 = CONJUNCT2 ARITH_ZERO in
+  let th_0 = (PURE_REWRITE_RULE [NUMERAL] o prove)
+   (`numbit i 0 = F`, REWRITE_TAC [numbit; DIV_0; ODD]) in
+  let th00,th01 = (CONJ_PAIR o PURE_REWRITE_RULE [NUMERAL] o prove)
+   (`numbit 0 (BIT0 n) = F /\ numbit 0 (BIT1 n) = T`,
+     REWRITE_TAC [numbit; EXP; DIV_1; ARITH_ODD]) in
+  let thS0,thS1 = (CONJ_PAIR o UNDISCH o prove) (`i = SUC j ==>
+    numbit i (BIT0 n) = numbit j n /\ numbit i (BIT1 n) = numbit j n`,
+    DISCH_THEN SUBST1_TAC THEN CONV_TAC BITS_ELIM_CONV THEN
+    REWRITE_TAC [numbit; EXP; GSYM DIV_DIV;
+      ARITH_RULE `(2 * n + 1) DIV 2 = n /\ (2 * n) DIV 2 = n`]) in
+  let thB1S = prove (`BIT1 i = SUC (BIT0 i)`, REWRITE_TAC [ARITH_SUC]) in
+  let thB10 = MATCH_MP (DISCH_ALL thS0) thB1S
+  and thB11 = MATCH_MP (DISCH_ALL thS1) thB1S in
+  let thSB1 = (UNDISCH o prove) (`i = SUC j ==> BIT0 i = SUC (BIT1 j)`,
+    DISCH_THEN SUBST1_TAC THEN REWRITE_TAC [ARITH_SUC]) in
+  let thB00 = PROVE_HYP thSB1 (INST [`BIT0 i`,i;`BIT1 j`,j] thS0)
+  and thB01 = PROVE_HYP thSB1 (INST [`BIT0 i`,i;`BIT1 j`,j] thS1) in
+  let th0B00,th0B01 =
+    let th = AP_TERM `numbit` (TRANS (AP_TERM `BIT0` (ASSUME `i = _0`)) B00) in
+    TRANS (AP_THM th `BIT0 n`) th00, TRANS (AP_THM th `BIT1 n`) th01 in
+  let thN = prove
+   (`numbit (NUMERAL i) (NUMERAL n) = numbit i n`, REWRITE_TAC [NUMERAL]) in
+  let get_suc th = Some (rand (rhs (concl th))), th in
+  let rec mk_pred = function
+  | Comb(Const("BIT0",_),i') ->
+    (match mk_pred i' with
+    | Some j', th -> get_suc (PROVE_HYP th (INST [i',i; j',j] thSB1))
+    | None, th -> None, TRANS (AP_TERM B0 th) B00)
+  | Comb(Const("BIT1",_),i') -> get_suc (INST [i',i] thB1S)
+  | Const("_0",_) as i' -> None, REFL i'
+  | _ -> failwith "BIT_PRED" in
+  let rec go = function
+  | i',Const("_0",_) -> INST [i',i] th_0
+  | Const("_0",_),Comb(Const("BIT0",_),n') -> INST [n',n] th00
+  | Const("_0",_),Comb(Const("BIT1",_),n') -> INST [n',n] th01
+  | Comb(Const("BIT0",_),i'),Comb(Const("BIT0",_),n') ->
+    go_B0 th0B00 thB00 i' n'
+  | Comb(Const("BIT0",_),i'),Comb(Const("BIT1",_),n') ->
+    go_B0 th0B01 thB01 i' n'
+  | Comb(Const("BIT1",_),i'),Comb(Const("BIT0",_),n') ->
+    TRANS (INST [i',i; n',n] thB10) (go (mk_comb (B0,i'),n'))
+  | Comb(Const("BIT1",_),i'),Comb(Const("BIT1",_),n') ->
+    TRANS (INST [i',i; n',n] thB11) (go (mk_comb (B0,i'),n'))
+  | _ -> failwith "NUMBIT_CONV"
+  and go_B0 th0 thS i' n' = match mk_pred i' with
+  | Some j',th ->
+    let th' = PROVE_HYP th (INST [i',i; j',j; n',n] thS) in
+    TRANS th' (go (mk_comb (B1,j'), n'))
+  | None, th -> PROVE_HYP th (INST [i',i; n',n] th0) in
+  mk_pred, function
+  | Comb(Comb(Const("numbit",_),
+      Comb(Const("NUMERAL",_),i')),Comb(Const("NUMERAL",_),n')) ->
+    TRANS (INST [i',i;n',n] thN) (go (i',n'))
+  | Comb(Comb(Const("numbit",_),i'),n') -> go (i',n')
+  | _ -> failwith "NUMBIT_CONV";;
+
+(* ------------------------------------------------------------------------- *)
+(* A primitive operation for splitting numerals along powers of 2.           *)
+(* ------------------------------------------------------------------------- *)
+
+let num_shift_add = new_definition
+  `num_shift_add a b n = a MOD 2 EXP n + b * 2 EXP n`;;
+
+let num_shift_add_0 = prove
+ (`num_shift_add a b 0 = b`,
+  REWRITE_TAC [num_shift_add; EXP; MOD_1; MULT_CLAUSES; ADD]);;
+
+let EXP_2_MOD_LT =
+  GEN_ALL (REWRITE_RULE [GSYM (SPEC `a:num` MOD_LT_EQ)] EXP_2_NE_0);;
+
+let num_shift_add_SUC = prove
+ (`num_shift_add (BIT0 a) b (SUC n) = BIT0 (num_shift_add a b n) /\
+   num_shift_add (BIT1 a) b (SUC n) = BIT1 (num_shift_add a b n)`,
+  REWRITE_TAC [num_shift_add; EXP] THEN CONV_TAC BITS_ELIM_CONV THEN
+  REWRITE_TAC [LEFT_ADD_DISTRIB; MOD_MULT2; MULT_AC] THEN
+  REWRITE_TAC [ADD_AC; EQ_ADD_LCANCEL] THEN
+  ONCE_REWRITE_TAC [SYM (MATCH_MP MOD_LT
+    (MATCH_MP (ARITH_RULE `a < b ==> a * 2 + 1 < b * 2`)
+      (SPECL [`a:num`;`n:num`] EXP_2_MOD_LT)))] THEN
+  ONCE_REWRITE_TAC [GSYM MOD_ADD_MOD] THEN
+  REWRITE_TAC [ONCE_REWRITE_RULE [MULT_SYM] MOD_MULT2; MOD_MOD_REFL]);;
+
+let num_shift_add_lt = prove
+ (`!a b n i. b < 2 EXP i ==> num_shift_add a b n < 2 EXP (i + n)`,
+  REPEAT GEN_TAC THEN REWRITE_TAC [num_shift_add; EXP_ADD] THEN
+  DISCH_TAC THEN MATCH_MP_TAC LTE_TRANS THEN EXISTS_TAC `SUC b * 2 EXP n` THEN
+  ASM_REWRITE_TAC [LE_MULT_RCANCEL; MULT_CLAUSES; ADD_SYM; LT_ADD_LCANCEL;
+    EXP_2_MOD_LT; LE_SUC_LT]);;
+
+let num_shift_add_mod = prove
+ (`num_shift_add a (b MOD 2 EXP i) n = num_shift_add a b n MOD 2 EXP (i + n)`,
+  ONCE_REWRITE_TAC [(SYM o MATCH_MP MOD_LT o SPEC_ALL)
+    (MATCH_MP num_shift_add_lt (SPECL [`b:num`; `i:num`] EXP_2_MOD_LT))] THEN
+  REWRITE_TAC [num_shift_add; EXP_ADD] THEN
+  ONCE_REWRITE_TAC [GSYM MOD_ADD_MOD] THEN
+  REWRITE_TAC [GSYM (ONCE_REWRITE_RULE [MULT_SYM] MOD_MULT2); MOD_MOD_REFL]);;
+
+(* (NUM_SHIFT_ADD_CONV `num_shift_add a b i`), and
+   (NUM_SHIFT_ADD_CORE `a` `b` `i`), will prove `|- num_shift_add a b i = n`
+   where a,b,i,n are numerals or raw numerals. *)
+
+let NUM_SHIFT_ADD_CORE, NUM_SHIFT_ADD_CONV =
+  let i,j,a,b,e = `i:num`,`j:num`,`a:num`,`b:num`,`e:num` in
+  let i0 = (UNDISCH o prove) (`i = _0 ==> num_shift_add a b i = b`,
+    DISCH_THEN SUBST1_TAC THEN CONV_TAC BITS_ELIM_CONV THEN
+    ACCEPT_TAC num_shift_add_0) in
+  let B0S,B1S = (CONJ_PAIR o UNDISCH_ALL o prove)
+   (`num_shift_add a b j = e ==> i = SUC j ==>
+    num_shift_add (BIT0 a) b i = BIT0 e /\
+    num_shift_add (BIT1 a) b i = BIT1 e`,
+    DISCH_THEN (SUBST1_TAC o SYM) THEN DISCH_THEN SUBST1_TAC THEN
+    REWRITE_TAC [num_shift_add_SUC]) in
+  let ZS = REWRITE_RULE [ARITH_ZERO] (INST [`_0`,a] B0S)
+  and B00 = REWRITE_RULE [ARITH_ZERO] (INST [`_0`,e] B0S) in
+  let Z0 = REWRITE_RULE [ARITH_ZERO] (INST [`_0`,e] ZS) in
+  let rec go a' b' i' = match BIT_PRED i' with
+  | None, th -> PROVE_HYP th (INST [i',i; a',a; b',b] i0)
+  | Some j', th ->
+    PROVE_HYP th (match a' with
+    | Comb(Const("BIT0",_),a') ->
+      let th' = go a' b' j' in
+      PROVE_HYP th' (match rhs (concl th') with
+      | Const("_0",_) -> INST [i',i; j',j; a',a; b',b] B00
+      | e' -> INST [e',e; i',i; j',j; a',a; b',b] B0S)
+    | Comb(Const("BIT1",_),a') ->
+      let th' = go a' b' j' in
+      let e' = rhs (concl th') in
+      PROVE_HYP th' (INST [e',e; i',i; j',j; a',a; b',b] B1S)
+    | Const("_0",_) ->
+      let th' = go a' b' j' in
+      PROVE_HYP th' (match rhs (concl th') with
+      | Const("_0",_) -> INST [i',i; j',j; a',a; b',b] Z0
+      | e' -> INST [e',e; i',i; j',j; a',a; b',b] ZS)
+    | _ -> failwith "NUM_SHIFT_ADD_CORE") in
+  let pthn = (UNDISCH o prove)
+   (`num_shift_add a b i = e ==>
+     num_shift_add (NUMERAL a) (NUMERAL b) (NUMERAL i) = NUMERAL e`,
+    REWRITE_TAC [NUMERAL]) in
+  go, function
+  | Comb(Comb(Comb(Const("num_shift_add",_), Comb(Const("NUMERAL",_),a')),
+      Comb(Const("NUMERAL",_),b')), Comb(Const("NUMERAL",_),i')) ->
+    let th = go a' b' i' in
+    PROVE_HYP th (INST [a',a; b',b; i',i; rhs (concl th),e] pthn)
+  | Comb(Comb(Comb(Const("num_shift_add",_),a'),b'),i') ->
+    go a' b' i'
+  | _ -> failwith "NUM_SHIFT_ADD_CONV";;
 
 (* ------------------------------------------------------------------------- *)
 (* Some "limiting" values with names in the style of C's "limits.h" macros.  *)
