Library/bitmatch.ml
@@ -1,0 +1,1168 @@
+(* ========================================================================= *)
+(*           Parsing and printing for bitmatch expressions.                  *)
+(*                                                                           *)
+(* This supports term constructions like                                     *)
+(*                                                                           *)
+(*   bitmatch (word 17) with                                                 *)
+(*   | [hi3:3; 0b00:2; lo3:3] -> foo hi3 lo3                                 *)
+(*   | [hi3:3; 0b1:1; lo4:4]  -> bar hi3 lo4                                 *)
+(*   | [0b1010101:7; b]       -> baz b                                       *)
+(*                                                                           *)
+(* which decomposes the number 17 = 0b00010001 into the 3 high bits          *)
+(* (hi3 = 0), a 1 bit in the middle, and the 4 low bits (lo4 = 1) and calls  *)
+(* `bar`.  The patterns are written with the low bits on the right.          *)
+(* A pattern variable without a digit matches one bit as a bool.             *)
+(*                                                                           *)
+(*                (c) Copyright, Mario Carneiro 2020                         *)
+(* ========================================================================= *)
+
+needs "Library/words.ml";;
+
+prioritize_num();;
+
+(* Like CHOOSE, but the variable is the same as the one in the existential *)
+
+let TRIV_CHOOSE =
+  let P = `P:A->bool` and Q = `Q:bool` and an = `(/\)` in
+  let pth = (* `(\x:A. Q /\ P x) = P, (?) P |- Q` *)
+    let th1 = AP_THM (ASSUME `(\x:A. Q /\ P x) = P`) `x:A` in
+    let th1 = TRANS (SYM th1) (BETA `(\x:A. Q /\ P x) x`) in
+    let th1 = CONJUNCT1 (EQ_MP th1 (ASSUME `(P:A->bool) x`)) in
+    let th1 = GEN `x:A` (DISCH `(P:A->bool) x` th1) in
+    let th2 = CONV_RULE (RAND_CONV BETA_CONV) (AP_THM EXISTS_DEF P) in
+    MP (SPEC `Q:bool` (EQ_MP th2 (ASSUME `(?) (P:A->bool)`))) th1 in
+  fun th1 th2 ->
+    try let P' = rand (concl th1) in
+        let v,bod = dest_abs P' in
+        let Q' = concl th2 in
+        let anQ = mk_comb (an, Q') in
+        let th3 = DEDUCT_ANTISYM_RULE (CONJ th2 (ASSUME bod))
+          (CONJUNCT2 (ASSUME (mk_comb (anQ, bod)))) in
+        let th4 = AP_TERM anQ (BETA (mk_comb (P', v))) in
+        let th5 = PINST [snd(dest_var v),aty] [P',P; Q',Q] pth in
+        PROVE_HYP th1 (PROVE_HYP (ABS v (TRANS th4 th3)) th5)
+    with Failure _ -> failwith "TRIV_CHOOSE";;
+
+let (WITH_GOAL:(term->tactic)->tactic) = fun tac (_,w as st) -> tac w st;;
+
+let _BITMATCH = new_definition `_BITMATCH (s:N word) c = _MATCH (val s) c`;;
+let _ELSEPATTERN = new_definition `_ELSEPATTERN (e:B) (a:A) = \x. e = x`;;
+
+let bitpat =
+  let th = prove
+    (`?x:num#(num->bool). !a. SND x a ==> a < 2 EXP FST x`,
+    EXISTS_TAC `0, \i:num. F` THEN REWRITE_TAC[SND]) in
+  new_type_definition "bitpat" ("mk_bitpat","dest_bitpat") th;;
+
+let pat_size = new_definition `pat_size p = FST (dest_bitpat p)`;;
+let pat_set = new_definition `pat_set p = SND (dest_bitpat p)`;;
+
+let pat_set_lt = prove (`!p s. pat_set p s ==> s < 2 EXP pat_size p`,
+  REWRITE_TAC [pat_set; pat_size; bitpat]);;
+
+let pat_thm = prove (`p = mk_bitpat (n, f) /\ (!a. f a ==> a < 2 EXP n) ==>
+  pat_size p = n /\ !s. pat_set p s = f s`,
+  REPEAT DISCH_TAC THEN
+  SUBGOAL_THEN `dest_bitpat (mk_bitpat (n,f)) = (n,f)`
+    (fun th -> ASM_REWRITE_TAC [pat_size; pat_set; th]) THEN
+  ASM_REWRITE_TAC [GSYM (CONJUNCT2 bitpat)] THEN
+  FIRST_X_ASSUM (ASSUME_TAC o MATCH_MP pat_set_lt));;
+
+let NILPAT = new_definition `NILPAT = mk_bitpat(0,\s:num. s = 0)`;;
+
+let NILPAT_pat_size,NILPAT_pat_set = (CONJ_PAIR o prove)
+ (`pat_size NILPAT = 0 /\ !s. pat_set NILPAT s <=> s = 0`,
+  MATCH_MP_TAC pat_thm THEN REWRITE_TAC [NILPAT] THEN
+  STRIP_TAC THEN DISCH_THEN SUBST1_TAC THEN ARITH_TAC);;
+
+let CONSPAT = new_definition `CONSPAT p (a:N word) =
+  let n = dimindex(:N) in
+  mk_bitpat(n + pat_size p,
+    \s:num. (?t. pat_set p t /\ s = val a + 2 EXP n * t))`;;
+
+let CONSPAT_pat_size,CONSPAT_pat_set = (CONJ_PAIR o prove)
+ (`pat_size (CONSPAT p (a:N word)) = dimindex(:N) + pat_size p /\
+   !s. pat_set (CONSPAT p (a:N word)) s <=>
+     ?t. pat_set p t /\ s = val a + 2 EXP dimindex(:N) * t`,
+  MATCH_MP_TAC pat_thm THEN
+  REWRITE_TAC [CONV_RULE (ONCE_DEPTH_CONV let_CONV) CONSPAT] THEN
+  REPEAT STRIP_TAC THEN POP_ASSUM SUBST1_TAC THEN
+  MATCH_MP_TAC LTE_TRANS THEN EXISTS_TAC `2 EXP dimindex (:N) * SUC t` THEN
+  POP_ASSUM (fun th -> REWRITE_TAC [EXP_ADD; LE_MULT_LCANCEL; LE_SUC_LT;
+    MATCH_MP pat_set_lt th]) THEN
+  REWRITE_TAC [MULT_SUC; LT_ADD_RCANCEL; VAL_BOUND]);;
+
+reserve_words["BITPAT"; "bitmatch"];;
+
+let word1 = new_definition `word1 p = (word (bitval p)):1 word`;;
+
+let BIT0_WORD1 = prove (`bit 0 (word1 b) = b`,
+  REWRITE_TAC [word1; BIT_LSB; bitval; VAL_WORD] THEN DIMINDEX_TAC THEN
+  BOOL_CASES_TAC `b:bool` THEN REWRITE_TAC [] THEN ARITH_TAC);;
+
+let VAL_WORD1 = prove (`val (word1 b) = bitval b`,
+  REWRITE_TAC [word1; VAL_WORD_BITVAL]);;
+
+let WORD1_ODD = prove (`word1 (ODD n) = word n`,
+  CONV_TAC SYM_CONV THEN REWRITE_TAC [word1; WORD_EQ; DIMINDEX_CLAUSES] THEN
+  ASM_CASES_TAC `ODD n` THEN
+  ASM_REWRITE_TAC[ODD_MOD; BITVAL_CLAUSES; EXP_1; CONG] THEN
+  CONV_TAC NUM_REDUCE_CONV THEN
+  ASM_REWRITE_TAC[GSYM EVEN_MOD; GSYM ODD_MOD; GSYM NOT_ODD]);;
+
+let preparse_bitpat,preparse_bitmatch =
+  let bitmatch_ptm = Varp("_BITMATCH",dpty)
+  and NILPAT_ptm = Varp("NILPAT",dpty)
+  and CONSPAT_ptm = Varp("CONSPAT",dpty)
+  and word_ptm = Varp("word",dpty)
+  and word1_ptm = Varp("word1",dpty)
+  and arb_ptm = Varp("ARB",dpty)
+  and ung_ptm = Varp("_UNGUARDED_PATTERN",dpty)
+  and seqp_ptm = Varp("_SEQPATTERN",dpty)
+  and else_ptm = Varp("_ELSEPATTERN",dpty) in
+  let rec pfrees ptm = match ptm with
+  | Varp(v,pty) ->
+      if v = "" && pty = dpty then []
+      else if can get_const_type v || can num_of_string v
+              || exists (fun (w,_) -> v = w) (!the_interface) then []
+      else [ptm]
+  | Constp(_,_) -> []
+  | Combp(p1,p2) -> union (pfrees p1) (pfrees p2)
+  | Absp(p1,p2) -> subtract (pfrees p2) (pfrees p1)
+  | Typing(p,_) -> pfrees p in
+  let pgenvar =
+    let gcounter = ref 0 in
+    fun () -> let count = !gcounter in
+              (gcounter := count + 1;
+               Varp("BM%PVAR%"^(string_of_int count),dpty)) in
+  let pmk_exists v ptm = Combp(Varp("?",dpty),Absp(v,ptm)) in
+  let pmk_bitmatch (((_,e),_),cs) =
+    let x = pgenvar() and y = pgenvar() in
+    let rec pmk_clauses cs = match pmk_clauses_opt cs with
+    | Some t -> t
+    | None -> Combp(else_ptm, arb_ptm)
+    and pmk_clauses_opt cs = match cs with
+    | [] -> None
+    | (None,res)::cs -> Some (Combp(else_ptm, res))
+    | (Some pat,res)::cs ->
+      let tx = Combp(Combp(Varp("pat_set",dpty),pat),x)
+      and ty = Combp(Combp(Varp("=",dpty),res),y) in
+      let t = itlist pmk_exists (pfrees pat) (Combp(Combp(ung_ptm,tx),ty)) in
+      Some(Combp(Combp(seqp_ptm, Absp(x, Absp(y, t))), pmk_clauses cs)) in
+    Combp(Combp(bitmatch_ptm,e), pmk_clauses cs) in
+  let rec to_bitpat p e = match e with
+  | Varp("NIL",_) -> p
+  | Combp(Combp(Varp("CONS",_),a),e) ->
+    let e2 = match a with
+    | Typing(a,i) ->
+        let a = match a with
+        | Varp(s,_) when can num_of_string s -> Combp(word_ptm,a)
+        | _ -> a in
+        Typing(a,Ptycon("word",[i]))
+    | a -> Combp(word1_ptm,a) in
+    to_bitpat (Combp(Combp(CONSPAT_ptm,p),e2)) e
+  | _ -> raise Noparse in
+  let bitpat = parse_preterm >> to_bitpat NILPAT_ptm in
+  let pattern = (a (Ident "_") >> (fun _ -> None))
+    ||| (bitpat >> fun x -> Some(x)) in
+  let clause = pattern ++ (a (Resword "->") ++ parse_preterm >> snd) in
+  let clauses =
+    possibly (a (Resword "|")) ++
+      listof clause (a (Resword "|")) "pattern-match clause" >> snd in
+  (a (Resword "BITPAT") ++ bitpat >> snd),
+  (a (Resword "bitmatch") ++ parse_preterm ++ a (Resword "with") ++ clauses
+    >> pmk_bitmatch);;
+
+install_parser("bitpat",preparse_bitpat);;
+install_parser("bitmatch",preparse_bitmatch);;
+
+let pp_print_bitpat,pp_print_bitmatch =
+  let rec dest_pat_rev tm =
+    match tm with
+    | Comb(Comb(Const("CONSPAT",_),p),a) -> a::dest_pat_rev p
+    | Const("NILPAT",_) -> []
+    | _ -> failwith "dest_pat" in
+  let dest_pat = rev o dest_pat_rev in
+  let dest_clause tm =
+    match snd(strip_exists(body(body tm))) with
+    | Comb(Comb(Const("_UNGUARDED_PATTERN",_),lhs),
+        Comb(Comb(Const("=",_),res),_)) ->
+      (match lhs with
+      | Comb(Comb(Const("pat_set",_),pat),_) -> dest_pat pat, res
+      | _ -> failwith "dest_clause")
+    | _ -> failwith "dest_clause" in
+  let rec dest_clauses tm =
+    match tm with
+    | Comb(Comb(Const("_SEQPATTERN",_),c),cs) ->
+        let c = dest_clause c and l,r = dest_clauses cs in c::l,r
+    | Comb(Const("_ELSEPATTERN",_),res) -> [],res
+    | _ -> failwith "dest_clauses" in
+  let f fmt =
+    let unword i = function
+    | Comb(Const("word",_),a) when is_numeral a ->
+      if dest_numeral a < power_num (Int 2) (dest_finty i)
+      then a
+      else failwith "numeral out of range"
+    | a -> a in
+    let print_pat = function
+    | Comb(Const("word1",_),a) -> pp_print_term fmt a
+    | a -> match type_of a with
+      | Tyapp("word",[i]) ->
+          (pp_print_term fmt (unword i a);
+          pp_print_string fmt ":";
+          pp_print_type fmt i)
+      | _ -> failwith "print_pat" in
+    let print_opat = function
+    | None -> pp_print_string fmt "_"
+    | Some [] -> pp_print_string fmt "[]"
+    | Some (x::xs) ->
+       (pp_print_string fmt "[";
+        print_pat x;
+        List.iter (fun x ->
+          pp_print_string fmt "; ";
+          print_pat x) xs;
+        pp_print_string fmt "]") in
+    let print_clause p r =
+      (print_opat p;
+       pp_print_string fmt " -> ";
+       pp_print_term fmt r) in
+    let rec print_clauses cls r = match cls,r with
+    | [p,res],Const("ARB",_) -> print_clause (Some p) res
+    | (p,res)::cs,_ -> (
+      print_clause (Some p) res;
+      pp_print_break fmt 1 0;
+      pp_print_string fmt "| ";
+      print_clauses cs r)
+    | [],r -> print_clause None r in
+    let pp_print_bitpat tm =
+      let pat = dest_pat tm in
+      (pp_open_hvbox fmt 0;
+       pp_print_string fmt "(BITPAT";
+       pp_print_space fmt ();
+       print_opat (Some pat);
+       pp_print_string fmt ")";
+       pp_close_box fmt ()) in
+    let pp_print_bitmatch = function
+    | Comb(Comb(Const("_BITMATCH",_),e),c) ->
+        let cls,r = dest_clauses c in
+        (pp_open_hvbox fmt 0;
+         pp_print_string fmt "(bitmatch ";
+         pp_print_term fmt e;
+         pp_print_string fmt " with";
+         pp_print_break fmt 1 2;
+         print_clauses cls r;
+         pp_close_box fmt ();
+         pp_print_string fmt ")")
+    | _ -> failwith "print_bitmatch" in
+    pp_print_bitpat,pp_print_bitmatch in
+  fst o f, snd o f;;
+
+let print_bitpat = pp_print_bitpat std_formatter
+and string_of_bitpat = print_to_string pp_print_bitpat;;
+
+let print_bitmatch = pp_print_bitmatch std_formatter
+and string_of_bitmatch = print_to_string pp_print_bitmatch;;
+
+install_user_printer("bitpat",pp_print_bitpat);;
+install_user_printer("bitmatch",pp_print_bitmatch);;
+
+(* ------------------------------------------------------------------------- *)
+(* Some tactics for dealing with bitmatch                                    *)
+(* ------------------------------------------------------------------------- *)
+
+let dest_word_ty = function
+| Tyapp("word",[i]) -> i
+| _ -> failwith "dest_word_ty";;
+
+let SPLIT_IF =
+  let th = (UNDISCH_ALL o TAUT)
+    `(p ==> a:A = t1) ==> (~p ==> a = t2) ==> a = if p then t1 else t2` in
+  let [Var(_,A) as a; p; t1; t2] = frees (concl th) and tnot = `~` in
+  fun p' th1 th2 ->
+    let a',t1' = dest_eq (concl th1) and
+    t2' = snd (dest_eq (concl th2)) in
+    (PROVE_HYP (DISCH p' th1) o PROVE_HYP (DISCH (mk_comb(tnot, p')) th2))
+    (PINST [type_of a',A] [p',p; a',a; t1',t1; t2',t2] th);;
+
+let MATCH_SEQPATTERN = prove
+ (`_MATCH (e:A) (_SEQPATTERN c cs) =
+   if ?y:B. c e y then _MATCH e c else _MATCH e cs`,
+  COND_CASES_TAC THEN ASM_REWRITE_TAC [_MATCH; _SEQPATTERN]);;
+
+let BITMATCH_SEQPATTERN = prove
+ (`_BITMATCH (e:N word) (_SEQPATTERN c cs) =
+   if ?y:B. c (val e) y then _BITMATCH e c else _BITMATCH e cs`,
+  REWRITE_TAC [_BITMATCH; MATCH_SEQPATTERN]);;
+
+let BITMATCH_SEQPATTERN2 = prove
+ (`_BITMATCH (e:N word) (_SEQPATTERN c cs) =
+   if ?y:B. c (val e) y then
+     _BITMATCH e (_SEQPATTERN c (_ELSEPATTERN ARB))
+   else _BITMATCH e cs`,
+  REWRITE_TAC [BITMATCH_SEQPATTERN] THEN COND_CASES_TAC THEN REWRITE_TAC []);;
+
+let MATCH_ELSEPATTERN = prove
+ (`_MATCH (e:B) (_ELSEPATTERN (a:A)) = a`,
+  REWRITE_TAC [_MATCH; _ELSEPATTERN] THEN METIS_TAC[]);;
+
+let BITMATCH_ELSEPATTERN = prove
+ (`_BITMATCH (e:N word) (_ELSEPATTERN (a:A)) = a`,
+  REWRITE_TAC [_BITMATCH; MATCH_ELSEPATTERN]);;
+
+let pat_extract = new_definition `pat_extract p i b <=>
+  (!n. pat_set p n ==> numbit i n = b)`;;
+
+let PAT_EXTRACT_THM =
+  let N,n,m,i,p,b = `:N`,`n:num`,`m:num`,`i:num`,`p:bitpat`,`b:bool`
+  and a,lt,pl,nb,di = `a:N word`,`(<)`,`(+)`,`numbit`,`dimindex(:N)` in
+  let word1_eq = prove
+   (`pat_extract (CONSPAT p (word1 b)) 0 b`,
+    REWRITE_TAC [pat_extract; numbit; CONSPAT_pat_set; word1; VAL_WORD] THEN
+    REPEAT STRIP_TAC THEN FIRST_X_ASSUM SUBST1_TAC THEN
+    DIMINDEX_TAC THEN NUM_REDUCE_TAC THEN
+    REWRITE_TAC [DIV_1; EVEN_ADD; GSYM NOT_EVEN; EVEN_DOUBLE] THEN
+    BOOL_CASES_TAC `b:bool` THEN REWRITE_TAC [bitval] THEN ARITH_TAC) in
+
+  let word_lt = (UNDISCH_ALL o prove)
+   (`dimindex(:N) = n ==> numbit i m = b ==> (i < n <=> T) ==>
+     pat_extract (CONSPAT p (word m:N word)) i b`,
+    REWRITE_TAC[] THEN REPEAT (DISCH_THEN (SUBST1_TAC o SYM)) THEN
+    REWRITE_TAC [pat_extract; CONSPAT_pat_set; numbit] THEN
+    REPEAT STRIP_TAC THEN FIRST_X_ASSUM SUBST1_TAC THEN
+    REWRITE_TAC [VAL_WORD; ODD_MOD; DIV_MOD] THEN
+    AP_THM_TAC THEN AP_TERM_TAC THEN AP_THM_TAC THEN AP_TERM_TAC THEN
+    ONCE_REWRITE_TAC [MULT_SYM] THEN
+    REWRITE_TAC [GSYM (CONJUNCT2 EXP)] THEN
+    ONCE_REWRITE_TAC [GSYM MOD_ADD_MOD] THEN
+    FIRST_X_ASSUM (SUBST1_TAC o GSYM o
+      MATCH_MP (ARITH_RULE `m <= n ==> (m + (n - m) = n:num)`) o
+      REWRITE_RULE [GSYM LE_SUC_LT]) THEN
+    REWRITE_TAC [EXP_ADD; MOD_MOD] THEN ONCE_REWRITE_TAC [MULT_AC] THEN
+    REWRITE_TAC [MOD_MULT; ADD_0; MOD_MOD_REFL]) in
+
+  let word_skip = (UNDISCH_ALL o prove)
+   (`dimindex(:N) = n ==> m + n = i ==> pat_extract p m b ==>
+     pat_extract (CONSPAT p (a:N word)) i b`,
+    REPEAT (DISCH_THEN (SUBST1_TAC o SYM)) THEN
+    REWRITE_TAC [pat_extract; CONSPAT_pat_set; numbit] THEN
+    REPEAT STRIP_TAC THEN FIRST_X_ASSUM SUBST1_TAC THEN
+    POP_ASSUM (fun th -> POP_ASSUM (fun f ->
+      REWRITE_TAC [GSYM (MATCH_MP f th)])) THEN
+    REWRITE_TAC [SPECL [m;`dimindex(:N)`] ADD_SYM] THEN
+    REWRITE_TAC [EXP_ADD; GSYM DIV_DIV] THEN
+    AP_TERM_TAC THEN AP_THM_TAC THEN AP_TERM_TAC THEN
+    IMP_REWRITE_TAC [DIV_MULT_ADD; DIV_LT; ADD; VAL_BOUND; EXP_2_NE_0]) in
+
+  let rec go = function
+  | Comb(Comb(Const("CONSPAT",_),p'),a'),i' ->
+    let i'' = dest_numeral i' in
+    let aty = type_of a' in
+    let Tyapp(_,[N']) = aty in
+    let n'' = dest_finty N' in
+    if i'' < n'' then
+      match a' with
+      | Comb(Const("word1",_),b') -> INST [p',p; b',b] word1_eq
+      | Comb(Const("word",_),m') when is_numeral m' ->
+        let th = INST_TYPE [N',N] word_lt in
+        let th1 = DIMINDEX_CONV (inst [N',N] di) in
+        let n' = rhs (concl th1) in
+        let th2 = NUMBIT_CONV (mk_comb (mk_comb (nb,i'),m')) in
+        let b' = rhs (concl th2) in
+        let th3 = NUM_LT_CONV (mk_comb (mk_comb (lt,i'),n')) in
+        (PROVE_HYP th3 o PROVE_HYP th2 o PROVE_HYP th1)
+          (INST [i',i; m',m; n',n; p',p; b',b] th)
+      | _ -> failwith "PAT_EXTRACT_THM: not a constant at this position"
+    else
+      let th = INST_TYPE [N',N] word_skip in
+      let th1 = DIMINDEX_CONV (inst [N',N] di) in
+      let n' = rhs (concl th1) in
+      let m' = mk_numeral (sub_num i'' n'') in
+      let th2 = NUM_ADD_CONV (mk_comb (mk_comb (pl,m'),n')) in
+      let th3 = go (p', m') in
+      let b' = rand (concl th3) in
+      (PROVE_HYP th3 o PROVE_HYP th2 o PROVE_HYP th1)
+        (INST [i',i; m',m; n',n; p',p; b',b; a',mk_var("a",aty)] th)
+  | _ -> failwith "PAT_EXTRACT_THM: out of range"
+  in go;;
+
+(* (pat_to_bit false `i` `pat_set p (val e)`) proves
+    `bit i e |- ~pat_set p (val e)` or
+    `~bit i e |- ~pat_set p (val e)`
+    (pat_to_bit true `i` `pat_set p (val e)`) proves
+    `pat_set p (val e) |- ~bit i e` or
+    `pat_set p (val e) |- bit i e` *)
+let pat_to_bit =
+  (* thT := ~bit i e, pat_extract p i T |- ~pat_set p (val e)
+      thF := bit i e, pat_extract p i F |- ~pat_set p (val e) *)
+  let thT_pos,thF_pos =
+    (* TODO: I got frustrated with tactics so this is just a direct proof. *)
+    let a = PURE_REWRITE_RULE [pat_extract] (ASSUME `pat_extract p i b`) in
+    let a = UNDISCH (SPEC `val (e:N word)` a) in
+    let th = TRANS (SYM NUMBIT_VAL) a in
+    EQT_ELIM (INST [`T`,`b:bool`] th), EQF_ELIM (INST [`F`,`b:bool`] th) in
+  let thT_neg,thF_neg =
+    let f x y = NOT_INTRO (DISCH `pat_set p (val (e:N word))`
+      (MP (NOT_ELIM x) y)) in
+    f (ASSUME `~bit i (e:N word)`) thT_pos,
+    f thF_pos (ASSUME `bit i (e:N word)`) in
+  let N,i,e,p = `:N`,`i:num`,`e:N word`,`p:bitpat` in
+  fun pos i' -> function
+  | Comb(Comb(Const("pat_set",_),p'),
+      Comb(Const("val",Tyapp(_,[Tyapp(_, [N']); _])),e')) ->
+    let thp = PAT_EXTRACT_THM (p', i') in
+    let th = match rand (concl thp) with
+    | Const("T",_) -> if pos then thT_pos else thT_neg
+    | Const("F",_) -> if pos then thF_pos else thF_neg
+    | _ -> failwith "pat_to_bit" in
+    PROVE_HYP thp (PINST [N',N] [i',i; e',e; p',p] th)
+  | _ -> failwith "pat_to_bit";;
+
+let bm_analyze_pat sz =
+  let A = Array.make sz None in
+  let rec go i = function
+  | Comb(Comb(Const("CONSPAT",_),p),a) ->
+    let n = Num.int_of_num (dest_finty (dest_word_ty (type_of a))) in
+    if i + n > sz then
+      raise (Invalid_argument "incorrect bit length") else
+    let () = match a with
+    | Comb(Const("word1",_),a) ->
+      A.(i) <- (match a with
+        | Const("T",_) -> Some true
+        | Const("F",_) -> Some false
+        | Var(_,_) -> None
+        | _ -> failwith "bm_analyze_pat")
+    | Comb(Const("word",_),Comb(Const("NUMERAL",_),a)) ->
+      let rec analyze_num n a = match a with
+      | Comb(Const("BIT0",_),a) ->
+        (A.(n) <- Some false; analyze_num (n+1) a)
+      | Comb(Const("BIT1",_),a) ->
+        (A.(n) <- Some true; analyze_num (n+1) a)
+      | Const("_0",_) -> Array.fill A n (sz - n) (Some false)
+      | _ -> failwith "bm_analyze_pat" in
+      analyze_num i a
+    | Var(_,_) -> Array.fill A i n None
+    | _ -> failwith "bm_analyze_pat" in
+    go (i + n) p
+  | Const("NILPAT",_) ->
+    if i = sz then () else
+    raise (Invalid_argument "incorrect bit length")
+  | Abs(_,c) -> go i c
+  | Comb(Const("?",_),c) -> go i c
+  | Comb(Comb(Const("_UNGUARDED_PATTERN",_),c),_) -> go i c
+  | Comb(Comb(Const("pat_set",_),c),_) -> go i c
+  | _ -> failwith "bm_analyze_pat" in
+  fun pat ->
+    try go 0 pat; A
+    with Invalid_argument _ -> failwith (sprintf
+      "bm_analyze_pat: pattern %s has incorrect bit length"
+      (string_of_term pat));;
+
+let rec bm_analyze_clauses sz = function
+| Comb(Comb(Const("_SEQPATTERN",_),c),cs) ->
+  let pat = (lhand o lhand o snd o strip_exists o body o body) c in
+  bm_analyze_pat sz pat :: bm_analyze_clauses sz cs
+| _ -> [];;
+
+(* (bm_skip_clause f `_BITMATCH e (_SEQPATTERN r rs)`) returns
+   `A |- _BITMATCH e (_SEQPATTERN r rs) = _BITMATCH e rs` if
+   (f `pat_set p (val e)`) proves `A |- ~pat_set p (val e)`
+   (probably via pat_to_bit false) *)
+let bm_skip_clause =
+  let th = (UNDISCH o prove)
+    (`(?) (r (val e)) = F ==>
+      (_BITMATCH e (_SEQPATTERN r rs):B) = _BITMATCH (e:N word) rs`,
+    REPEAT DISCH_TAC THEN REWRITE_TAC [BITMATCH_SEQPATTERN] THEN
+    CONV_TAC (ONCE_DEPTH_CONV ETA_CONV) THEN ASM_REWRITE_TAC []) in
+  let N,B,e,r,rs =
+    `:N`,`:B`,`e:N word`,`r:num->B->bool`,`rs:num->B->bool` in
+
+  (* (strip_ex `x` `A |- P[x] = F`) proves `A |- (?x. P[x]) = F` *)
+  let strip_ex =
+    let th1 = (UNDISCH o prove)
+      (`(P = \x:A. F) ==> (?) P = F`, DISCH_TAC THEN ASM_REWRITE_TAC[]) in
+    let A = `:A` and P = `P:A->bool` in
+    fun x th ->
+      let th' = ABS x th in
+      PROVE_HYP th' (PINST [type_of x,A] [lhs (concl th'),P] th1) in
+
+  (* (skip_guard `A` `B`) proves `~A |- _UNGUARDED_PATTERN A B = F` *)
+  let skip_guard =
+    let th = (UNDISCH o prove)
+      (`~A ==> _UNGUARDED_PATTERN A B = F`,
+      DISCH_TAC THEN ASM_REWRITE_TAC [_UNGUARDED_PATTERN]) in
+    let A = `A:bool` and B = `B:bool` in
+    fun A' B' -> INST [A',A; B',B] th in
+
+  fun f -> function
+  | Comb(Comb(Const("_BITMATCH",ty),e'),
+      Comb(Comb(Const("_SEQPATTERN",_),c),rs')) ->
+    let Tyapp(_, [N']),Tyapp(_, [_; B']) = dest_fun_ty ty in
+    let th = PINST [N',N;B',B] [e',e; c,r; rs',rs] th in
+    let ex,h = dest_comb (lhs (hd (hyp th))) in
+    let th2 = BETA_CONV h in
+    let th3 = AP_TERM ex th2 in
+    let rec skip_exs = function
+    | Comb(Const("?",_),Abs(y,c)) -> strip_ex y (skip_exs c)
+    | Comb(Comb(Const("_UNGUARDED_PATTERN",_),p),res) ->
+      PROVE_HYP (f p) (skip_guard p res)
+    | _ -> failwith "skip_exs" in
+    PROVE_HYP (TRANS th3 (skip_exs (rhs (concl th3)))) th
+  | _ -> failwith "bm_skip_clause";;
+
+type 'a discrim_tree =
+    Leaf_dt of 'a
+  | Split_dt of int * term * 'a discrim_tree * 'a discrim_tree;;
+
+let rec map_dt f = function
+| Leaf_dt a -> Leaf_dt (f a)
+| Split_dt(i, bit, tr1, tr2) ->
+  Split_dt(i, bit, map_dt f tr1, map_dt f tr2);;
+
+let bm_build_tree' =
+  let bit_tm =
+    let N = `:N` in
+    fun i e ->
+      let Tyapp("word",[N']) = type_of e in
+      let bit = mk_const("bit",[N',N]) in
+      mk_comb(mk_comb(bit,i),e) in
+
+  (* (seqp_rand `r` `A |- _BITMATCH e rs1 = _BITMATCH e rs2`) proves
+     `A |- _BITMATCH e (_SEQPATTERN r rs1) =
+           _BITMATCH e (_SEQPATTERN r rs2)` *)
+  let seqp_rand =
+    let th = (UNDISCH o prove)
+      (`_BITMATCH (e:N word) (rs1:num->B->bool) = _BITMATCH e rs2 ==>
+        _BITMATCH e (_SEQPATTERN r rs1) = _BITMATCH e (_SEQPATTERN r rs2)`,
+      DISCH_TAC THEN ASM_REWRITE_TAC [BITMATCH_SEQPATTERN]) in
+    let [rs1; e; r; rs2] = frees (concl th) and N,B = `:N`,`:B` in
+    fun r' th' ->
+      match dest_eq (concl th') with
+      | Comb(Comb(Const(_,ty),e'),rs1'),Comb(_,rs2') ->
+      let Tyapp(_, [N']),Tyapp(_, [_; B']) = dest_fun_ty ty in
+      PROVE_HYP th' (PINST [N',N; B',B] [e',e; r',r; rs1',rs1; rs2',rs2] th)
+      | _ -> failwith "seqp_rand" in
+
+  let aMerge a b = match a,b with
+  | None,_ -> a
+  | _,None -> None
+  | Some(a0,a1),Some false -> Some(a0+1, a1)
+  | Some(a0,a1),Some true -> Some(a0, a1+1) in
+
+  fun sz cls -> function
+  | Comb(Comb(Const("_BITMATCH",_),e) as m, cs) as tm ->
+    let rec build eqth cls cs =
+      let analysis = Array.make sz (Some(0,0)) in
+      let _ = List.iter (Array.iteri
+        (fun i a -> analysis.(i) <- aMerge analysis.(i) a)) cls in
+      let r =
+        let r = ref None in
+        let f i a = match a with
+        | Some(n1,n2) when n1 != 0 && n2 != 0 ->
+          let v = abs (n1 - n2) in
+          (match !r with
+          | Some(v',_) when v' <= v -> ()
+          | _ -> r := Some(v, i))
+        | _ -> () in
+        (Array.iteri f analysis; !r) in
+      match r with
+      | None -> Leaf_dt eqth
+      | Some(_,i) ->
+        let ii = mk_numeral (Int i) in
+        let bit = bit_tm ii e in
+        let skip_th sc th =
+          let sm, rs' = dest_comb (lhs (concl th)) in
+          let tm = mk_comb (sm, mk_comb (sc, rs')) in
+          TRANS (bm_skip_clause (pat_to_bit false ii) tm) th in
+        let rec split_ths = function
+        | [], cs -> let th = REFL (mk_comb(m,cs)) in [],[],th,th
+        | cl::cls, Comb(Comb(Const("_SEQPATTERN",_),c) as sc,cs) ->
+          let cls1,cls2,th1,th2 = split_ths(cls, cs) in
+          if let Some(b) = cl.(i) in b then
+            cls1, cl::cls2, skip_th sc th1, seqp_rand c th2
+          else
+            cl::cls1, cls2, seqp_rand c th1, skip_th sc th2
+        | cl::cls, cs ->
+          let cls1,cls2,th1,th2 = split_ths(cls, cs) in
+          if let Some(b) = cl.(i) in b then
+            cls1, cl::cls2, th1, th2
+          else
+            cl::cls1, cls2, th1, th2
+        | _ -> failwith "split_ths" in
+        let cls1,cls2,th1,th2 = split_ths(cls, cs) in
+        let tr1 = build (TRANS eqth th1) cls1 (rand (rhs (concl th1)))
+        and tr2 = build (TRANS eqth th2) cls2 (rand (rhs (concl th2))) in
+        Split_dt(i, bit, tr1, tr2) in
+    build (REFL tm) cls cs
+  | _ -> failwith "bm_build_tree'";;
+
+let bm_build_tree = function
+| Comb(Comb(Const("_BITMATCH",_),e),cs) as tm ->
+  let sz = Num.int_of_num (dest_finty (dest_word_ty (type_of e))) in
+  let cls = bm_analyze_clauses sz cs in
+  cls, bm_build_tree' sz cls tm
+| _ -> failwith "bm_build_tree";;
+
+let BM_IF_CONV =
+  let rec of_tree = function
+  | Leaf_dt th -> th
+  | Split_dt(_, bit, tr1, tr2) -> SPLIT_IF bit (of_tree tr2) (of_tree tr1) in
+  of_tree o snd o bm_build_tree;;
+
+let MATCH_EQ = prove
+ (`(r:A->B->bool) e = (\y. x = y) ==> _MATCH e r = x`,
+  REWRITE_TAC [_MATCH] THEN DISCH_THEN SUBST1_TAC THEN METIS_TAC[]);;
+
+let bitpat_inverts = new_definition
+ `bitpat_inverts p f (x:A) <=> (!y. pat_set p y ==> f y = x)`;;
+
+let bitpat_down = new_definition
+ `bitpat_down(:N) (f:num->A) (n:num) = f (n DIV 2 EXP dimindex(:N))`;;
+
+let CONSPAT_down_inverts = prove
+ (`bitpat_inverts p f (x:A) ==>
+   bitpat_inverts (CONSPAT p (a:N word)) (bitpat_down(:N) f) x`,
+  REWRITE_TAC [bitpat_inverts; bitpat_down; CONSPAT_pat_set] THEN
+  REPEAT STRIP_TAC THEN FIRST_X_ASSUM MATCH_MP_TAC THEN
+  FIRST_X_ASSUM SUBST1_TAC THEN
+  IMP_REWRITE_TAC [DIV_MULT_ADD; DIV_LT; VAL_BOUND; EXP_2_NE_0] THEN
+  ASM_REWRITE_TAC [ADD]);;
+
+let CONSPAT_word_inverts = prove
+ (`bitpat_inverts (CONSPAT p (a:N word)) word a`,
+  REWRITE_TAC [bitpat_inverts; CONSPAT_pat_set] THEN
+  REPEAT STRIP_TAC THEN FIRST_X_ASSUM SUBST1_TAC THEN
+  REWRITE_TAC [WORD_VAL_GALOIS; MOD_MULT_ADD] THEN
+  REWRITE_TAC [GSYM WORD_VAL_GALOIS; WORD_VAL]);;
+
+let bitpat_inverts_comp = MESON [bitpat_inverts; o_DEF]
+ `bitpat_inverts p f (x:A) ==> bitpat_inverts p (g o f) (g x:B)`;;
+
+let CONSPAT_word1_inverts =
+  (* `bitpat_inverts (CONSPAT p (word1 b)) (bit 0 o word) b` *)
+  REWRITE_RULE [BIT0_WORD1]
+    (PART_MATCH rand (MATCH_MP bitpat_inverts_comp CONSPAT_word_inverts)
+      (lhs (concl BIT0_WORD1)));;
+
+(* Given a pattern `p` and a target variable `z`,
+  (build_inverts `p`) produces an association list mapping `z`
+  to `|- bitpat_inverts p f z` for some term `f` not containing `z`. *)
+let build_inverts =
+  let N,A,p,a,f,x,b =
+    `:N`,`:A`,`p:bitpat`,`a:N word`,`f:num->A`,`x:A`,`b:bool`
+  and th0 = ASSUME `bitpat_inverts p f (x:A)`
+  and th1 = UNDISCH CONSPAT_down_inverts in
+  let rec go = function
+  | Const("NILPAT",_),_ -> []
+  | (Comb(Comb(Const("CONSPAT",_),p'),a') as cp),thunk ->
+    let Tyapp(_, [N']) = type_of a' in
+    let next th =
+      let th' = PINST [N',N] [a',a] th1 in
+      let Comb(Comb(_,p'),f') = rator (concl th') in
+      PROVE_HYP th' (INST [p',p; f',f] th) in
+    let var v thv =
+      let th = thunk() in
+      let f' = rand (rator (concl thv)) in
+      let th' = PROVE_HYP thv (PINST [type_of v,A] [cp,p; f',f; v,x] th) in
+      (v,th') :: go (p', fun () -> next th) in
+    (match a' with
+    | Var(_,_) -> var a' (PINST [N',N] [p',p; a',a] CONSPAT_word_inverts)
+    | Comb(Const("word1",_), (Var(_,_) as b')) ->
+      var b' (INST [p',p; b',b] CONSPAT_word1_inverts)
+    | _ -> go (p', next o thunk))
+  | _ -> failwith "build_inverts" in
+  fun p' -> go (p', fun () -> th0);;
+
+
+(* Given `bitmatch e with p -> res | ...` proves
+   `bit_set p (val e) |- (bitmatch e with p -> res | ...) = res`,
+  and given `bitmatch e with _ -> res` proves
+  `(bitmatch e with _ -> res) = res`. *)
+let BM_FIRST_CASE_CONV =
+  let th1 = (UNDISCH o prove)
+   (`r (val (e:N word)) = (\y:A. x = y) ==> _BITMATCH e (_SEQPATTERN r s) = x`,
+    DISCH_TAC THEN
+    ASM_REWRITE_TAC [BITMATCH_SEQPATTERN; _BITMATCH; MESON[] `?y:A. x=y`] THEN
+    POP_ASSUM (ACCEPT_TAC o MATCH_MP MATCH_EQ)) in
+  let th2 = (UNDISCH o METIS[_UNGUARDED_PATTERN])
+    `A ==> (_UNGUARDED_PATTERN A B <=> B)` in
+  let th3 = EQ_MP (SYM th2) (ASSUME `B:bool`) in
+  let th4 = (UNDISCH_ALL o prove)
+   (`bitpat_inverts p f (x:A) ==> pat_set p e ==> f e = x`,
+    DISCH_THEN (MATCH_ACCEPT_TAC o REWRITE_RULE [bitpat_inverts])) in
+  let thg1,thg2 = (CONJ_PAIR o UNDISCH o METIS[_UNGUARDED_PATTERN])
+    `_UNGUARDED_PATTERN A B ==> A /\ B` in
+  let nty,eA,eB,ep,ef,ex = `:N`,`A:bool`,`B:bool`,`p:bitpat`,`f:num->A`,`x:A`
+  and ee,ea,er,es = `e:N word`,`a:A`,`r:num->A->bool`,`s:num->A->bool` in
+  function
+  | Comb(Comb(Const("_BITMATCH",_),e),
+      Comb(Comb(Const("_SEQPATTERN",_), (Abs(x,Abs(y,c')) as c)),cs)) as tm ->
+    let A' = type_of tm in
+    let N = dest_word_ty (type_of e) in
+    let val_e = mk_comb (mk_const("val", [N,nty]), e) in
+    let zs, Comb(Comb(Const("_UNGUARDED_PATTERN",_),
+      (Comb((Comb(_,p) as mp),_) as ps)),restm) = strip_exists c' in
+    let res = lhand restm in
+    let instAB = INST [ps,eA; restm,eB] in
+    let ps' = mk_comb (mp, val_e) in
+    let th' = if zs = [] then instAB th2 else
+      let inverts = build_inverts p in
+      let rec prove_ex c1 pr eqth = match c1 with
+      | Comb(Const("?",_),Abs(z,c')) ->
+        let inv = assoc z inverts in
+        let f = lhand (concl inv) in
+        let inv = PROVE_HYP inv (PINST [type_of z,aty]
+          [p,ep; f,ef; z,ex; x,`e:num`] th4) in
+        let abr = mk_abs (z, lhs (concl eqth)) in
+        let eqth1 = TRANS (AP_TERM abr (ASSUME (concl inv)))
+          (BETA (mk_comb (abr, z))) in
+        let pr',th = prove_ex c' (PROVE_HYP inv o pr) (TRANS eqth1 eqth) in
+        pr', TRANS (SYM eqth1) (TRIV_CHOOSE (ASSUME c1) th)
+      | _ -> pr, TRANS (PROVE_HYP (instAB thg1) (pr eqth)) (instAB thg2) in
+      let pr,thR = prove_ex c' I (REFL res) in
+      DEDUCT_ANTISYM_RULE (itlist SIMPLE_EXISTS zs (instAB th3)) (pr thR) in
+    let th' = INST [val_e,x] (TRANS (BETA (mk_comb (c, x))) (ABS y th')) in
+    PROVE_HYP th' (PINST [N,nty; A',aty]
+      [e,ee; res,ex; c,er; cs,es] th1)
+  | Comb(Comb(Const("_BITMATCH",_),e), Comb(Const("_ELSEPATTERN",_), a)) ->
+    let A' = type_of a in
+    let N = dest_word_ty (type_of e) in
+    PINST [N,nty; A',aty] [e,ee; a,ea] BITMATCH_ELSEPATTERN
+  | _ -> failwith "BM_FIRST_CASE_CONV";;
+
+let bm_add_pos tr = function
+| Comb(Comb(Const("_BITMATCH",_),e),cs) ->
+  let N = dest_word_ty (type_of e) in
+  let val_e = mk_comb (mk_const("val", [N,`:N`]), e) in
+  let rec build_cases stk mth = function
+  | Comb(Comb(Const("_SEQPATTERN",_), Abs(x,Abs(y,c'))),cs) ->
+    let ps' = mk_comb (rator (lhand (snd (strip_exists c'))), val_e) in
+    let th = itlist (fun n ->
+      try PROVE_HYP (pat_to_bit true n ps') with Failure _ -> I) stk mth in
+    TRANS th (BM_FIRST_CASE_CONV (rhs (concl th))) :: build_cases stk mth cs
+  | _ -> [] in
+  let rec build stk = function
+  | Leaf_dt mth ->
+    Leaf_dt (mth, build_cases stk mth (rand (rhs (concl mth))))
+  | Split_dt (i, bit, tr1, tr2) ->
+    let stk' = lhand bit :: stk in
+    Split_dt (i, bit, build stk' tr1, build stk' tr2) in
+  build [] tr
+| _ -> failwith "bm_build_pos_tree";;
+
+let bm_build_pos_tree tm =
+  let A, tr = bm_build_tree tm in A, bm_add_pos tr tm;;
+
+let rec get_dt A = function
+| Leaf_dt a -> [], a
+| Split_dt(i, bit, tr1, tr2) ->
+  match A.(i) with
+  | None -> failwith ("get_dt splitting on " ^ string_of_int i)
+  | Some b ->
+    let stk,r = get_dt A (if b then tr2 else tr1) in
+    (b,bit)::stk, r;;
+
+let BM_CASES tm =
+  let A, tr = bm_build_pos_tree tm in
+  map (fun cl -> hd (snd (snd (get_dt cl tr)))) A;;
+
+(* (bitpat_matches `p` n) returns None if the pattern `p` would match
+   `word n`, and Some(i) where i is the smallest differing bit otherwise.
+   It throws if n >= 2^pat_size p. *)
+let rec bitpat_matches p i = match p with
+| Comb(Comb(Const("CONSPAT",_),p),a) ->
+  let N = dest_word_ty (type_of a) in
+  let n = Num.int_of_num (dest_finty N) in
+  let m = power_num (Int 2) (Int n) in
+  let i' = quo_num i m and a' = mod_num i m in
+  let r = match a with
+  | Comb(Const("word1",_),Const("T",_)) -> if a' = Int 1 then None else Some 0
+  | Comb(Const("word1",_),Const("F",_)) -> if a' = Int 0 then None else Some 0
+  | Comb(Const("word1",_),Var(_,_)) -> None
+  | Comb(Const("word",_),n) ->
+    let n' = dest_numeral n in
+    if a' = n' then None else
+    let rec f i r = if i land 1 != 0 then r else f (i lsr 1) (r+1) in
+    Some (f ((Num.int_of_num a') lxor (Num.int_of_num n')) 0)
+  | Var(_,_) -> None
+  | _ -> failwith "bitpat_matches" in
+  (match r with
+  | Some j -> Some j
+  | None ->
+    match bitpat_matches p i' with
+    | Some j -> Some (j + n)
+    | None -> None)
+| Const("NILPAT",_) -> if i = Int 0 then None else
+  failwith "bitpat_matches: out of range"
+| Abs(_,c) -> bitpat_matches c i
+| Comb(Const("?",_),c) -> bitpat_matches c i
+| Comb(Comb(Const("_UNGUARDED_PATTERN",_),c),_) -> bitpat_matches c i
+| Comb(Comb(Const("pat_set",_),c),_) -> bitpat_matches c i
+| _ -> failwith "bitpat_matches";;
+
+(* (inst_bitpat_numeral `pat_set p (val e)` n) will produce an instantiation
+   theta for p and e such that e[theta] = word n, and a proof of
+    `|- (pat_set p (val e))[theta]`.
+
+   (inst_bitpat_numeral `pat_set p e` n) will produce an instantiation
+   theta for p and e such that e[theta] = n, and a proof of
+    `|- (pat_set p e)[theta]`. *)
+let inst_bitpat_numeral =
+  let en,ep,ex,ei,ea = `n:num`,`p:bitpat`,`x:num`,`i:num`,`a:num`
+  and eN,T,F = `:N`,`T`,`F` in
+  let dim =
+    let dN = `dimindex(:N)` in
+    fun N -> DIMINDEX_CONV (inst [N,eN] dN) in
+
+  let w0 = prove (`pat_set NILPAT _0`,
+    REWRITE_TAC [NILPAT_pat_set; NUMERAL])
+  and wS,(w1T,w1F) =
+    let pth = prove
+     (`pat_set p x ==>
+       pat_set (CONSPAT p (word a:N word)) (num_shift_add a x (dimindex(:N)))`,
+      REWRITE_TAC [CONSPAT_pat_set; num_shift_add] THEN
+      DISCH_THEN (fun th ->
+        EXISTS_TAC ex THEN REWRITE_TAC [th; VAL_WORD; MULT_SYM])) in
+    (UNDISCH_ALL o prove)
+     (`dimindex(:N) = NUMERAL n ==> num_shift_add a x n = i ==> pat_set p x ==>
+       pat_set (CONSPAT p (word (NUMERAL a):N word)) i`,
+      REWRITE_TAC [NUMERAL] THEN
+      REPEAT (DISCH_THEN (SUBST1_TAC o SYM)) THEN ACCEPT_TAC pth),
+    (CONJ_PAIR o UNDISCH o prove)
+     (`pat_set p x ==>
+       pat_set (CONSPAT p (word1 T)) (BIT1 x) /\
+       pat_set (CONSPAT p (word1 F)) (BIT0 x)`,
+      REWRITE_TAC [word1; bitval] THEN
+      DISCH_THEN (fun th -> CONJ_TAC THEN ASSUME_TAC th) THENL [
+        POP_ASSUM (MP_TAC o MP (PINST [`:1`,eN] [`1`,ea] pth)) THEN
+        SUBGOAL_THEN
+          `num_shift_add 1 x (dimindex(:1)) = num_shift_add (BIT1 0) x (SUC 0)`
+          (fun th -> REWRITE_TAC [th; num_shift_add_SUC; num_shift_add_0]) THEN
+        CONV_TAC (ONCE_DEPTH_CONV DIMINDEX_CONV) THEN
+        REWRITE_TAC [BIT1_0; ONE];
+        POP_ASSUM (MP_TAC o MP (PINST [`:1`,eN] [`0`,ea] pth)) THEN
+        SUBGOAL_THEN
+          `num_shift_add 0 x (dimindex(:1)) = num_shift_add (BIT0 0) x (SUC 0)`
+          (fun th -> REWRITE_TAC [th; num_shift_add_SUC; num_shift_add_0]) THEN
+        CONV_TAC (ONCE_DEPTH_CONV DIMINDEX_CONV) THEN
+        REWRITE_TAC [BIT0_0; ONE]]) in
+  let w1F0 = REWRITE_RULE [ARITH_ZERO] (INST [`_0`,ex] w1F) in
+
+  let rec go i = function
+  | Comb(Comb(Const("CONSPAT",_),p),a) ->
+    let N = dest_word_ty (type_of a) in
+    let n = Num.int_of_num (dest_finty N) in
+    let m = power_num (Int 2) (Int n) in
+    let i' = quo_num i m and a' = mod_num i m in
+    let ls, th' = go i' p in
+    let p',x = dest_comb (concl th') in let p' = rand p' in
+    (match a with
+    | Comb(Const("word1",_),a) ->
+      let ls, b = match a with
+      | Const("T",_) -> ls,true
+      | Const("F",_) -> ls,false
+      | Var(_,_) -> let b = a' = Int 1 in ((if b then T else F),a)::ls, b
+      | _ -> failwith "inst_bitpat_numeral" in
+      ls, PROVE_HYP th' (
+        if b then INST [x,ex; p',ep] w1T
+        else if i = Int 0 then INST [p',ep] w1F0
+        else INST [x,ex; p',ep] w1F)
+    | _ ->
+      let thd = dim N in
+      let n' = rand (rhs (concl thd)) in
+      let ls, a = match a with
+      | Comb(Const("word",_),Comb(Const("NUMERAL",_),a)) -> ls, a
+      | Var(_,_) ->
+        let n = mk_numeral a' in
+        (mk_comb (mk_const ("word", [N,eN]), n), a) :: ls, rand n
+      | _ -> failwith "inst_bitpat_numeral" in
+      let thn = NUM_SHIFT_ADD_CORE a x n' in
+      let e = rhs (concl thn) in
+      ls, PROVE_HYP th' (PROVE_HYP thn (PROVE_HYP thd
+        (INST [n',en; a,ea; x,ex; e,ei; p',ep] (INST_TYPE [N,eN] wS)))))
+  | Const("NILPAT",_) -> [], w0
+  | _ -> failwith "inst_bitpat_numeral" in
+
+  let pth1 = SYM (SPEC en NUMERAL)
+  and pth2 = (UNDISCH_ALL o prove)
+   (`pat_size p = NUMERAL n ==> dimindex(:N) = NUMERAL n ==>
+     pat_set p x ==> pat_set p (val (word (NUMERAL x):N word))`,
+    DISCH_THEN (SUBST1_TAC o SYM) THEN REPEAT STRIP_TAC THEN
+    REWRITE_TAC [NUMERAL] THEN IMP_REWRITE_TAC [VAL_WORD_EQ] THEN
+    POP_ASSUM (ACCEPT_TAC o MATCH_MP pat_set_lt))
+  and conv =
+    let ps = `pat_size` in
+    REWRITE_CONV [CONSPAT_pat_size; NILPAT_pat_size] THENC
+    ONCE_DEPTH_CONV DIMINDEX_CONV THENC REDEPTH_CONV NUM_ADD_CONV o
+    mk_comb o (fun tm -> (ps, tm)) in
+
+  let check p i = match bitpat_matches p i with
+  | None -> go i p
+  | _ -> failwith "inst_bitpat_numeral: number does not match pattern" in
+
+  function
+  | Comb(Comb(Const("pat_set",_),p), Comb(Const("val",_), e)) ->
+    let N' = dest_word_ty (type_of e) in
+    let thd = dim N' in
+    let pth2 = (PROVE_HYP thd o PROVE_HYP (conv p) o
+       INST [p,ep; rand (rhs (concl thd)),en] o INST_TYPE [N',eN]) pth2 in
+    fun i ->
+      let ls, th = check p i in
+      let e' = rand (concl th) in
+      let th1 = PROVE_HYP th (INST ((e',ex)::ls) pth2) in
+      (match e with
+      | Var(_,_) -> (rand (rand (concl th1)),e)::ls, th1
+      | _ when aconv e (rand (rand (concl th1))) -> ls, th1
+      | _ -> failwith "inst_bitpat_numeral: pattern failed")
+  | Comb(Comb(Const("pat_set",_),p), e) ->
+    fun i ->
+      let ls, th = check p i in
+      let f, e' = dest_comb (concl th) in
+      let th1 = INST [e',en] pth1 in
+      let th2 = EQ_MP (AP_TERM f th1) th in
+      (match e with
+      | Var(_,_) -> (rhs (concl th1), e)::ls, th2
+      | _ when aconv e (rhs (concl th1)) -> ls, th2
+      | _ -> failwith "inst_bitpat_numeral: pattern failed")
+  | _ -> failwith "inst_bitpat_numeral";;
+
+let BITMATCH_CONV =
+  fun tm -> match tm with
+  | Comb(Comb(Const("_BITMATCH",_),
+      Comb(Const("word",Tyapp(_,[_;Tyapp(_,[N])])),n)),_) when is_numeral n ->
+    let A, tr = bm_build_pos_tree tm in
+    let n = Num.int_of_num (dest_numeral n)
+    and sz = Num.int_of_num (dest_finty N) in
+    let a = Array.init sz (fun i -> Some (n land (1 lsl i) != 0)) in
+    (match snd (snd (get_dt a tr)) with
+    | th::_ ->
+      let ps = hd (hyp th) in
+      let ls, th' = inst_bitpat_numeral ps (Int n) in
+      PROVE_HYP th' (INST ls th)
+    | _ -> failwith "BITMATCH_CONV")
+  | _ -> failwith "BITMATCH_CONV";;
+
+let BITMATCH_SIMP_CONV asl =
+  let pos,neg =
+    let rec go = function
+    | [] -> [],[]
+    | th::ths ->
+      let pos,neg = go ths in
+      match concl th with
+      | Comb(Const("~",_),c) when
+        (match snd (strip_exists c) with
+        | Comb(Comb(Const("pat_set",_),_),_) -> true
+        | _ -> false) -> pos,th::neg
+      | Comb(Comb(Const("pat_set",_),_),_) -> th::pos,neg
+      | _ -> pos,neg in
+    go asl in
+  let rec conv = function
+  | Comb(Comb(Const("_BITMATCH",_),_),Comb(Const("_ELSEPATTERN",_),_)) as tm ->
+    PART_MATCH lhs BITMATCH_ELSEPATTERN tm
+  | Comb(Comb(Const("_BITMATCH",_),
+      Comb(Const("word",_),n)),_) as tm when is_numeral n -> BITMATCH_CONV tm
+  | Comb(Comb(Const("_BITMATCH",_),e),
+      Comb(Comb(Const("_SEQPATTERN",_),c),cs)) as tm ->
+    let pat = mk_comb (rator (lhand (snd (strip_exists (body (body c))))),
+        mk_comb (mk_const ("val", [dest_word_ty (type_of e),`:N`]), e)) in
+    let vars = frees (lhand pat) in
+    let rec check_pos = function
+    | th::ths -> (try
+        let _,ls,_ = term_unify vars pat (concl th) in
+        PROVE_HYP th (INST ls (BM_FIRST_CASE_CONV tm))
+      with Failure _ -> check_pos ths)
+    | [] ->
+      let rec check_neg = function
+      | th::ths -> (try
+          let pat' = snd (strip_exists (rand (concl th))) in
+          let _,ls,_ = term_unify (frees (lhand pat')) pat' pat in
+          let ath = INST ls (SPEC_ALL
+            (PURE_REWRITE_RULE [NOT_EXISTS_THM] (ASSUME (concl th)))) in
+          let th' = PROVE_HYP th (bm_skip_clause (K ath) tm) in
+          TRANS th' (TRY_CONV conv (rhs (concl th')))
+        with Failure _ -> check_neg ths)
+      | [] ->
+        let sz = Num.int_of_num (dest_finty (dest_word_ty (type_of e))) in
+        let a = bm_analyze_pat sz pat in
+        let rec check_disj = function
+        | th::ths -> (try
+            let h = concl th in
+            let a' = bm_analyze_pat sz h in
+            let r = ref None in
+            Array.iteri (fun i x -> match x,a'.(i),!r with
+              | Some b, Some c, None when b != c -> r := Some i
+              | _ -> ()) a;
+            let i = match !r with
+            | Some i -> mk_numeral (Int i)
+            | _ -> fail () in
+            let th' = PROVE_HYP th (PROVE_HYP (pat_to_bit true i h)
+              (bm_skip_clause (pat_to_bit false i) tm)) in
+            TRANS th' (TRY_CONV conv (rhs (concl th')))
+          with Failure _ -> check_disj ths)
+        | [] -> failwith "BITMATCH_SIMP_CONV" in
+        check_disj pos in
+      check_neg neg in
+    check_pos pos
+  | _ -> failwith "BITMATCH_SIMP_CONV" in
+  conv;;
+
+let rec bitpat_irrefutable = function
+| Comb(Comb(Const("CONSPAT",_),p),a) ->
+  (match a with
+  | Comb(Const("word1",_),Var(_,_)) -> bitpat_irrefutable p
+  | Var(_,_) -> bitpat_irrefutable p
+  | _ -> false)
+| Const("NILPAT",_) -> true
+| Abs(_,c) -> bitpat_irrefutable c
+| Comb(Const("?",_),c) -> bitpat_irrefutable c
+| Comb(Comb(Const("_UNGUARDED_PATTERN",_),c),_) -> bitpat_irrefutable c
+| Comb(Comb(Const("pat_set",_),c),_) -> bitpat_irrefutable c
+| _ -> failwith "bitpat_irrefutable";;
+
+let bitpat_irrefutable_thm =
+  let eN,ee,ee',en,em,ek = `:N`,`e:num`,`e:N word`,`n:num`,`m:num`,`k:num`
+  and ep,dN,pl,_1 = `p:bitpat`,`dimindex(:N)`,`(+)`,`1`
+  and e2n = `e DIV 2 EXP n`
+  and pth,pth1 =
+    let pth = prove
+     (`dimindex(:N) = n ==> pat_set p (e DIV 2 EXP n) ==>
+       pat_set (CONSPAT p (word e:N word)) e`,
+      REWRITE_TAC [CONSPAT_pat_set] THEN DISCH_THEN (SUBST1_TAC o SYM) THEN
+      DISCH_THEN (fun th -> EXISTS_TAC `e DIV 2 EXP dimindex(:N)` THEN
+        REWRITE_TAC [th; VAL_WORD; ADD_SYM; MULT_SYM;
+          GSYM (MATCH_MP DIVISION (SPEC `n:num` EXP_2_NE_0))])) in
+    UNDISCH_ALL pth,
+    (UNDISCH o prove)
+     (`pat_set p (e DIV 2 EXP 1) ==> pat_set (CONSPAT p (word1 (ODD e))) e`,
+      REWRITE_TAC [WORD1_ODD] THEN
+      ACCEPT_TAC (MATCH_MP pth (DIMINDEX_CONV `dimindex(:1)`)))
+  and pth0 = (UNDISCH o prove) (`e < 2 EXP 0 ==> pat_set NILPAT e`,
+    REWRITE_TAC [EXP; ARITH_RULE `n < 1 <=> n = 0`; NILPAT_pat_set])
+  and pthS = (UNDISCH_ALL o prove) (`n + m = k ==>
+    e < 2 EXP k ==> e DIV 2 EXP n < 2 EXP m`,
+    DISCH_THEN (SUBST1_TAC o SYM) THEN
+    IMP_REWRITE_TAC [EXP_ADD; RDIV_LT_EQ; EXP_2_NE_0])
+  and pthW = (UNDISCH_ALL o prove)
+   (`dimindex(:N) = n ==> val (e:N word) < 2 EXP n`,
+    DISCH_THEN (SUBST1_TAC o SYM) THEN REWRITE_TAC [VAL_BOUND]) in
+
+  let rec build = function
+  | Const("NILPAT",_),e -> [], INST [e,ee] pth0
+  | Comb(Comb(Const("CONSPAT",_),p),v),e ->
+    let pthS n m =
+      let th = NUM_ADD_CONV (mk_comb (mk_comb (pl, n), m)) in
+      PROVE_HYP th (INST [n,en; m,em; rhs (concl th),ek; e,ee] pthS) in
+    (match v with
+    | Comb(Const("word1",_),(Var(_,_) as v)) ->
+      let ls, th = build (p, vsubst [e,ee; _1,en] e2n) in
+      let th' = PROVE_HYP th (INST [lhand (concl th),ep; e,ee] pth1) in
+      (rand (rand (lhand (concl th'))),v)::ls,
+      PROVE_HYP (pthS _1 (rand (rand (hd (hyp th))))) th'
+    | Var(_,ty) ->
+      let N = dest_word_ty ty in
+      let th1 = DIMINDEX_CONV (inst [N,eN] dN) in
+      let n = rhs (concl th1) in
+      let ls, th = build (p, vsubst [e,ee; n,en] e2n) in
+      let th' = PROVE_HYP th1
+        (INST [n,en; lhand (concl th),ep; e,ee] (INST_TYPE [N,eN] pth)) in
+      let th' = PROVE_HYP th th' in
+      (rand (lhand (concl th')),v)::ls,
+      PROVE_HYP (pthS n (rand (rand (hd (hyp th))))) th'
+    | _ -> failwith "bitpat_irrefutable_thm: not irrefutable")
+  | _ -> failwith "bitpat_irrefutable_thm" in
+
+  fun tm -> match snd (strip_exists tm) with
+  | Comb(Comb(Const("pat_set",_),p),(Comb(Const("val",_),e') as e)) ->
+    let ls,th = build (p, e) in
+    let rec build_ex = function
+    | Comb(Const("?",_),Abs(v,c)) as tm ->
+      let e = rev_assoc v ls in
+      EXISTS (tm, e) (build_ex (vsubst [e,v] c))
+    | tm when aconv (concl th) tm -> th
+    | _ -> failwith "bitpat_irrefutable_thm: nonlinear pattern" in
+    let th = build_ex tm in
+    let N = dest_word_ty (type_of e') in
+    let th1 = DIMINDEX_CONV (inst [N,eN] dN) in
+    let n = rhs (concl th1) in
+    if aconv n (rand (rand (hd (hyp th)))) then
+      PROVE_HYP (PROVE_HYP th1 (PINST [N,eN] [n,en; e',ee'] pthW)) th
+    else failwith "bitpat_irrefutable_thm: incorrect bit length"
+  | _ -> failwith "bitpat_irrefutable_thm";;
+
+let ONLY_BITMATCH_CASES_THEN thltac = WITH_GOAL (fun w ->
+  let e,cs =
+    let f = function
+    | Comb(Comb(Const("_BITMATCH",_),_),_) -> true
+    | _ -> false in
+    (rand F_F I) (dest_comb (find_term f w)) in
+  let rec tac thl = function
+  | Comb(Comb(Const("_SEQPATTERN",_),Abs(_,Abs(_,c))),cs) ->
+    let rec go = function
+    | Comb((Const("?",_) as f),Abs(z,c)) ->
+      let tm, tac1 = go c in
+      mk_comb (f, mk_abs (z, tm)), POP_ASSUM CHOOSE_TAC THEN tac1
+    | tm ->
+      mk_comb (rator (lhand tm),
+        mk_comb (mk_const ("val", [dest_word_ty (type_of e),`:N`]), e)),
+      ALL_TAC in
+    let tm, tac1 = go c in
+    if bitpat_irrefutable c then
+      ASSUME_TAC (bitpat_irrefutable_thm tm) THEN
+      tac1 THEN POP_ASSUM (fun th -> thltac (th::thl))
+    else
+      ASM_CASES_TAC tm THENL [
+        tac1 THEN POP_ASSUM (fun th -> thltac (th::thl));
+        POP_ASSUM (fun th -> tac (th::thl) cs)]
+  | _ -> thltac thl in
+  tac [] cs);;
+
+let BITMATCH_ASM_CASES_TAC =
+  ONLY_BITMATCH_CASES_THEN (fun thl ->
+    CONV_TAC (TOP_SWEEP_CONV (BITMATCH_SIMP_CONV thl)) THEN
+    MAP_EVERY ASSUME_TAC thl);;
+
+let BITMATCH_CASES_TAC =
+  ONLY_BITMATCH_CASES_THEN (CONV_TAC o
+    TOP_SWEEP_CONV o BITMATCH_SIMP_CONV);;
+
+(* (bm_seq_numeral `bitmatch e with ...` n) will
+   return `word n` and `(bitmatch word n with ...) = res` where `res` is the
+   appropriate match branch. Unlike BITMATCH_CONV this also works with matches
+   with non-disjoint cases. *)
+let bm_seq_numeral = function
+| Comb((Comb(Const("_BITMATCH",_),e) as me),cs) ->
+  let N = dest_word_ty (type_of e) in
+  let sz = Num.int_of_num (dest_finty N) in
+  let word = mk_const ("word", [N,`:N`]) in
+  let rec mk_fun cs =
+    let tm = mk_comb (me, cs) in
+    let th = BM_FIRST_CASE_CONV tm in
+    let inst e' th = if is_var e then INST [e',e] th else th in
+    match cs with
+    | Comb(Comb(Const("_SEQPATTERN",_),c),cs') ->
+      let ps = hd (hyp th) in
+      let pats = Array.init sz (fun i -> try
+        Some (bm_skip_clause (pat_to_bit false (mk_numeral (Int i))) tm)
+      with Failure _ -> None) in
+      let f = mk_fun cs' in
+      fun n e' ->
+        (match bitpat_matches c n with
+        | None ->
+          let ls, th' = inst_bitpat_numeral ps n in
+          PROVE_HYP th' (INST ls th)
+        | Some i ->
+          let Some th' = pats.(i) in
+          let th1 = inst e' th' in
+          let th2 = match hd (hyp th1) with
+          | Comb(Const("~",_),p) -> EQF_ELIM (WORD_RED_CONV p)
+          | p -> EQT_ELIM (WORD_RED_CONV p) in
+          TRANS (PROVE_HYP th2 th1) (f n e'))
+    | Comb(Const("_ELSEPATTERN",_),_) -> fun _ e' -> inst e' th
+    | _ -> failwith "bm_seq_numeral" in
+  let f = mk_fun cs in
+  fun n -> let e = mk_comb (word, mk_numeral n) in e, f n e
+| _ -> failwith "bm_seq_numeral";;
+
+let BITMATCH_SEQ_CONV = function
+| Comb(Comb(Const("_BITMATCH",_), Comb(Const("word",_),n)),_) as tm ->
+  snd (bm_seq_numeral tm (dest_numeral n))
+| _ -> failwith "BITMATCH_CONV";;
